Softmax: slight generalization, some comments

src/klas/Klas.Softmax.fsti
@@ -3,10 +3,30 @@ module Klas.Softmax
 #lang-pulse
 open Kuiper
 module K = Kuiper.Kernel.Softmax
+open Kuiper.Array1
+open Kuiper.Tensor.Layout.Alg { l1_forward }
 
-val softmax_gpu_n_f16 : K.softmax_gpu_ty f16
-val softmax_gpu_n_f32 : K.softmax_gpu_ty f32
-val softmax_gpu_n_f64 : K.softmax_gpu_ty f64
+inline_for_extraction noextract
+type softmax_gpu_flat_ty (et : Type0) {| floating et, real_like et, floating_real_like et |} =
+  fn (nth : szp{nth <= max_threads})
+    (#lena : szp)
+    (a : array1 et (l1_forward lena) { is_global a })
+    (#va: erased (lseq et lena))
+    (ra: erased (lseq real lena))
+    preserves
+      cpu
+    requires
+      on gpu_loc (a |-> va) **
+      pure (va %~ ra) **
+      pure (lena <= max_blocks * max_threads)
+    ensures
+      exists* (va' : lseq et lena).
+        on gpu_loc (a |-> va') **
+        pure (va' %~ K.softmax_real ra)
+
+val softmax_gpu_n_f16 : softmax_gpu_flat_ty f16
+val softmax_gpu_n_f32 : softmax_gpu_flat_ty f32
+val softmax_gpu_n_f64 : softmax_gpu_flat_ty f64
 
 val softmax_n_f16 : K.softmax_ty f16
 val softmax_n_f32 : K.softmax_ty f32
