src/lib/kernel/Kuiper.Kernel.Softmax.fst
@@ -1,12 +1,12 @@
 module Kuiper.Kernel.Softmax
 
-(* Much of this module is layout-polymorphic, but
-we fix to l1_forward at the end so we can use arr_read_1. This
-should not be the case once there are more flexible memcpy's. *)
-
-// This is a very naive implementation of softmax on the GPU,
-// which uses three separate kernels launches (exp, reduce, divide).
-// A fused version is possible.
+(* Softmax, in two kernel calls.
+   1. Compute sum of exps (does not modify array)
+   2. Exp and divide by sum. Note: we are callng exp twice for every value.  An
+   alernative would be to first do an exp pass, then reduce, then divide, but I
+   think the extra kernel launch would be more expensive than the redundant
+   exp's.
+   *)
 
 #lang-pulse
 
@@ -35,7 +35,8 @@ fn softmax_gpu
   (#et : Type0) {| floating et, real_like et, floating_real_like et |}
   (nth : szp{nth <= max_threads})
   (#lena : szp)
-  (a : array1 et (l1_forward lena) { is_global a })
+  (#l : Array1.layout lena) {| ctlayout l |}
+  (a : array1 et l { is_global a })
   (#va: erased (lseq et lena))
   (ra: erased (lseq real lena))
   preserves
@@ -54,11 +55,12 @@ fn softmax_gpu
   assert pure (Seq.equal (seq_map id (seq_map rexp ra)) (seq_map rexp ra));
   let sum = Kuiper.Kernel.HReduce.reduce exp rexp nth lena a ra;
 
-  (* Exp and divide by sum. Note: we are callng exp twice for every value.  An
-  alernative would be to first do an exp pass, then reduce, then divide, but I
-  think the extra kernel launch would be more expensive than the redundant
-  exp's. *)
+  (* Exp and divide by sum. *)
   Kuiper.Kernel.Map.map_gpu (fun x -> div (exp x) sum) lena a;
+
+  (* Note: this could also be fused into a single kcall. The comfortable way of
+     doing that would require extensible barrier contracts, so we can add one more
+     step to the barrier of HReduce. *)
 
   softmax_approx va ra sum;
   ()
